Problem with modeling callbakc sequential calls

src/Primitive/Boolean/VstEnc.v
@@ -75,31 +75,53 @@ Definition bool_der_encode_spec : ident * funspec :=
          cb_p : val, 
          app_key_p : val,
          (* overrun callback destination buffer *)
-         buf_p : val
+         buf_p : val, buf_size : Z, computed_size : Z
     PRE [tptr enc_rval_s, tptr type_descriptor_s, tptr tvoid, tint, 
          tuint, tptr cb_type, tptr tvoid]
-      PROP (decoder_type td = BOOLEAN_t) 
+      PROP (decoder_type td = BOOLEAN_t;
+            isptr(buf_p)) 
       PARAMS (res; td_p; sptr_p; Vint (Int.repr tag_mode);
              Vint (Int.repr tag); cb_p; app_key_p)
       GLOBALS ()
-      SEP (data_at_ Tsh enc_rval_s res;
+      SEP (
+           (if buf_size <? computed_size + size
+            then emp 
+            else memory_block Tsh size (offset_val computed_size buf_p));
+           data_at_ Tsh enc_rval_s res;
            data_at_ Tsh type_descriptor_s td_p; 
            data_at Tsh tint (Vint sptr_val) sptr_p;
-           data_at Tsh enc_key_s (mk_enc_key sptr_p 3 0) app_key_p;
+           data_at Tsh enc_key_s (mk_enc_key buf_p buf_size computed_size) 
+                   app_key_p;
            valid_pointer cb_p;          
            func_ptr' callback cb_p)
     POST [tvoid]
       PROP ()
       LOCAL ()
       SEP (let res_val := 
-               match evalErrW (bool_encoder td (bool_of_int sptr_val)) [] with
-               | Some v => mk_enc_rval (encoded v) Vzero
-               | None => mk_enc_rval (-1) sptr_p
-               end in
+               match evalErrW (bool_encoder td (bool_of_int sptr_val)) [] with 
+                          | Some v => mk_enc_rval (encoded v) Vzero 
+                          | None => mk_enc_rval (-1) sptr_p end in
            data_at Tsh enc_rval_s res_val res;
            data_at_ Tsh type_descriptor_s td_p; 
            data_at Tsh tint (Vint sptr_val) sptr_p;
-           data_at Tsh enc_key_s (mk_enc_key sptr_p 3 3) app_key_p;
+           (* In the end we're know result, so we don't need size anymore *)
+           let tags_len := 
+               match evalErrW (Exec.der_write_tags td) [] with
+               | Some v => encoded v
+               | None => 0 end in 
+           (let arr := 
+               match execErrW (bool_encoder td (bool_of_int sptr_val)) [] with 
+               | Some res => res
+               | None => [] end in
+           (let size := if Zlength arr =? 0 then tags_len else Zlength arr in
+           (if buf_size <? computed_size + size
+            then data_at Tsh enc_key_s 
+                         (mk_enc_key buf_p 0 (computed_size + size)) app_key_p
+            else (data_at Tsh (tarray tuchar computed_size) (map Vubyte arr) 
+                          (offset_val computed_size buf_p) * 
+                  data_at Tsh enc_key_s 
+                          (mk_enc_key buf_p buf_size (computed_size + size))    
+                          app_key_p))));
            valid_pointer cb_p; 
            func_ptr' callback cb_p).
 
@@ -109,7 +131,9 @@ Definition Gprog := ltac:(with_library prog [der_write_tags_spec;
 
 Definition if_post1 cb_p sptr_p res bool_p erval_p td_p tag_mode 
            tag app_key_p td sptr_val cb_spec buf_p buf_size computed_size := 
-  PROP(is_pointer_or_null (cb_p))
+  PROP(is_pointer_or_null(cb_p)
+       (* der_write_tags writes 2 tags(bytes) to buffer *)
+       (*computed_size = (computed_size + 2)%Z*))
   LOCAL(temp _t'6 (Vint (Int.repr 2)); 
         temp _t'1 (Vint (Int.repr (encoded {| encoded := 2 |}))); 
         temp _st sptr_p; lvar _bool_value tuchar bool_p;
@@ -120,7 +144,18 @@ Definition if_post1 cb_p sptr_p res bool_p erval_p td_p tag_mode
         temp _cb (cb_p); temp _app_key app_key_p) 
   SEP(data_at_ Tsh type_descriptor_s td_p; 
       data_at_ Tsh enc_rval_s res; 
-      data_at Tsh enc_key_s (mk_enc_key buf_p buf_size computed_size) app_key_p;
+      let arr := match execErrW (Exec.der_write_tags td) [] with
+                 | Some r => r
+                 | None => [] end in
+      let size := Zlength arr in
+      (if buf_size <? computed_size + size
+       then data_at Tsh enc_key_s 
+                    (mk_enc_key buf_p 0 (computed_size + size)) app_key_p
+       else (data_at Tsh (tarray tuchar computed_size) (map Vubyte arr) 
+                     (offset_val computed_size buf_p) * 
+             data_at Tsh enc_key_s 
+                     (mk_enc_key buf_p buf_size (computed_size + size))    
+                     app_key_p));
       func_ptr' cb_spec (cb_p); 
       (match (cb_p) with
        | Vint _ => data_at_ Tsh tuchar bool_p
@@ -140,9 +175,9 @@ Definition if_post1 cb_p sptr_p res bool_p erval_p td_p tag_mode
       valid_pointer (cb_p)).
 
 Definition if_post2 sptr_val app_key_p v_bool_value cb_spec cb_p v_erval 
-           td_p res sptr_p tag_mode tag buf_p buf_size computed_size := 
+           td_p res sptr_p tag_mode tag buf_p buf_size computed_size size := 
   PROP()
-  LOCAL( temp _t'6 (Vint (Int.repr 2));
+  LOCAL(temp _t'6 (Vint (Int.repr 2));
         temp _t'1 (Vint (Int.repr (encoded {| encoded := 2 |}))); 
         temp _st sptr_p; lvar _bool_value tuchar v_bool_value;
         lvar _erval (Tstruct _asn_enc_rval_s noattr) v_erval; 
@@ -151,22 +186,32 @@ Definition if_post2 sptr_val app_key_p v_bool_value cb_spec cb_p v_erval
         temp _tag (Vint (Int.repr tag)); 
         temp _cb (cb_p); temp _app_key app_key_p;
         temp _t'2 (Vint (Int.repr (if (bool_of_int sptr_val) then 255 else 0))))
-  SEP(data_at_ Tsh type_descriptor_s td_p;
-      data_at Tsh enc_key_s (mk_enc_key buf_p buf_size computed_size) app_key_p;
-      func_ptr' cb_spec (cb_p);
+  SEP(if buf_size <? computed_size + size 
+      then data_at Tsh enc_key_s (mk_enc_key buf_p 0 computed_size) app_key_p 
+      else data_at Tsh (tarray tuchar 2) (map Vubyte [1%byte; 1%byte]) 
+                   (offset_val computed_size buf_p) * 
+           data_at Tsh enc_key_s (mk_enc_key buf_p buf_size (computed_size + 2)) 
+                   app_key_p; 
+      (if buf_size <? computed_size + size2
+       then emp
+       else memory_block Tsh size2 (offset_val computed_size buf_p));
+      data_at_ Tsh type_descriptor_s td_p; func_ptr' cb_spec cb_p;
       data_at_ Tsh tuchar v_bool_value;
-      field_at Tsh (Tstruct _asn_enc_rval_s noattr) (DOT _encoded) 
-               (Vint (Int.repr 2)) v_erval;
-      field_at Tsh (Tstruct _asn_enc_rval_s noattr) (DOT _failed_type) 
-               (default_val (tptr (Tstruct _asn_TYPE_descriptor_s noattr))) 
-               v_erval;
-      field_at Tsh (Tstruct _asn_enc_rval_s noattr) (DOT _structure_ptr) 
-               (default_val (tptr tvoid)) v_erval; 
-      data_at_ Tsh enc_rval_s res;
-      data_at Tsh tint (Vint sptr_val) sptr_p; valid_pointer (cb_p)).
+      field_at Tsh (Tstruct _asn_enc_rval_s noattr)
+                (DOT _encoded) (Vint (Int.repr 2)) v_erval;
+      field_at Tsh (Tstruct _asn_enc_rval_s noattr)
+                (DOT _failed_type)
+                 (default_val
+                     (tptr (Tstruct _asn_TYPE_descriptor_s noattr)))
+                  v_erval;
+      field_at Tsh (Tstruct _asn_enc_rval_s noattr)
+                (DOT _structure_ptr) (default_val (tptr tvoid))
+                 v_erval; data_at_ Tsh enc_rval_s res;
+      data_at Tsh tint (Vint sptr_val) sptr_p;
+      valid_pointer cb_p).
 
 Definition loop_inv sptr_p v_bool_value v_erval res td_p tag_mode tag cb_p 
-           app_key_p cb_spec sptr_val buf_p buf_size computed_size :=
+           app_key_p cb_spec sptr_val buf_p buf_size computed_size size :=
   PROP()
   LOCAL(temp _t'4 (Vint (Int.repr 2)); 
         temp _t'6 (Vint (Int.repr 2)); temp _t'1 (Vint (Int.repr 2)); 
@@ -179,6 +224,9 @@ Definition loop_inv sptr_p v_bool_value v_erval res td_p tag_mode tag cb_p
   SEP(data_at_ Tsh type_descriptor_s td_p;
       data_at_ Tsh enc_rval_s res; 
       data_at Tsh enc_key_s (mk_enc_key buf_p buf_size computed_size) app_key_p;
+      (if buf_size <? computed_size + size 
+       then emp 
+       else memory_block Tsh 1 (offset_val 2 buf_p));
       func_ptr' cb_spec (cb_p);
       data_at Tsh tuchar (Vubyte (byte_of_bool (bool_of_int sptr_val))) v_bool_value;
       field_at Tsh (Tstruct _asn_enc_rval_s noattr) (DOT _encoded) 
@@ -196,33 +244,46 @@ Theorem bool_der_encode : semax_body Vprog Gprog
                                                          composites)
                                      bool_der_encode_spec.
 Proof.
-  start_function; rename H into DT.
+  start_function; rename H into DT; rename H0 into Bf_ptr.
   forward.
   (* TODO specify data array with der_write_tags output *)
-  forward_call (td_p, td, 1, tag_mode, 0, tag, cb_p, app_key_p, 2, 
-                [Int.one; Int.one], td_p, buf_p, 3, 0).
+  forward_call (td_p, td, 1, tag_mode, 0, tag, cb_p, app_key_p, buf_p, buf_size, 
+                computed_size).
   
-  rewrite Exec.eval_dwt_boolean by assumption.
+  rewrite Exec.eval_dwt_boolean by assumption; 
+    rewrite Exec.exec_dwt_boolean by assumption; unfold encoded.
   unfold_data_at_ v_erval; unfold_data_at (data_at _ _ _ v_erval).
   forward.
   forward.
   forward_if; [contradiction|clear H].
   forward_if (if_post1 cb_p sptr_p res v_bool_value v_erval td_p tag_mode tag 
-                       app_key_p td sptr_val callback); unfold if_post1.
+                       app_key_p td sptr_val callback buf_p buf_size computed_size); 
+    unfold if_post1.
   * (* if(cb) = true *)
     forward.
     (* bool_value = *st ? 0xff : 0; /* 0xff mandated by DER */ *)
     forward_if (if_post2 sptr_val app_key_p v_bool_value callback cb_p v_erval 
-                         td_p res sptr_p tag_mode tag); unfold if_post2.
+                         td_p res sptr_p tag_mode tag buf_p buf_size 
+                         computed_size 2 size); unfold if_post2.
     - (* if(b) = true *)
-      forward; unfold if_post2; entailer!.
+      Intros size.
+      forward; unfold if_post2; Exists size; entailer!.
       unfold bool_of_int.
       destruct (sptr_val == 0)%int eqn : S; 
         [eapply int_eq_e in S; contradiction | auto ].
     - (* if(b) = false *)
-      forward; unfold if_post2; entailer!.
-    - forward.
-      forward_call ([sptr_val], v_bool_value, 1, app_key_p, buf_p, 3, 2).
+      Intros size.
+      forward; unfold if_post2; Exists size; entailer!.
+    - 
+      Intros size.
+      forward.
+      rewrite <-data_at_tuchar_singleton_array_eq.
+      forward_call ([(Int.zero_ext 8 (Int.repr (if bool_of_int sptr_val 
+                                                then 255 
+                                                else 0)))], 
+                    v_bool_value, 1, app_key_p, buf_p, buf_size, computed_size).
+      entailer!.
+      cbn.
       forward_if; [congruence|].
       ** (* cb() >= 0 *)
         unfold if_post1; forward.
