src/Lib/DWT/Vst.v
@@ -60,9 +60,8 @@ Definition der_write_tags_spec : ident * funspec :=
        (* callback pointer *)
        cb_p : val,
        (* callback argument pointer *)
-       app_p : val, size : Z,
+       app_p : val,
        (* overrun_encoder_key fields *)
-       data : list int, data_p : val,
        buf_p : val, buf_size : Z, computed_size : Z
   PRE[tptr type_descriptor_s, tuint, tint, tint, tuint, 
       tptr cb_type, tptr tvoid]
@@ -80,10 +79,24 @@ Definition der_write_tags_spec : ident * funspec :=
                                   | Some w => encoded w
                                   | None => -1
                                   end))))
-      SEP(data_at_ Tsh type_descriptor_s td_p ; 
-          data_at Tsh enc_key_s 
-                  (mk_enc_key buf_p buf_size (computed_size + size)) 
-                  app_p;
+      SEP(let res := evalErrW (der_write_tags td) [] in 
+          let size := match res with    
+                      | Some v => encoded v 
+                      | None => 0 end in
+          let res_ := execErrW (der_write_tags td) [] in
+          let arr := match res_ with
+                     | Some r => r
+                     | None => [] end in
+          (if buf_size <? computed_size + size
+           then data_at Tsh enc_key_s 
+                   (mk_enc_key buf_p 0 computed_size) app_p
+           else 
+             (data_at Tsh (tarray tuchar size) (map Vubyte arr) 
+                      (offset_val computed_size buf_p) *
+              data_at Tsh enc_key_s 
+                      (mk_enc_key buf_p buf_size (computed_size + size)) 
+                      app_p));
+          data_at_ Tsh type_descriptor_s td_p ; 
           func_ptr' callback cb_p).
 
 Definition Gprog := ltac:(with_library prog [der_write_tags_spec]).
